Work on Endianess.

src/BinEncoders/Env/Lib2/WordOpt.v
@@ -294,3 +294,278 @@ Proof.
     rewrite transform_push_step_opt, transform_push_pop_opt.
     rewrite IHsz; eauto.
 Qed.
+
+Section Word_little_endian.
+  Context {sz : nat}.
+
+  Context {B : Type}.
+  Context {cache : Cache}.
+  Context {cacheAddNat : CacheAdd cache nat}.
+  Context {transformer : Transformer B}.
+  Context {transformerUnit : TransformerUnitOpt transformer bool}.
+
+  Fixpoint encode_word' (s : nat) (w : word s) (b : B) : B :=
+    match w with
+    | WO => b
+    | WS b s' w' => (@encode_word' s' w')
+    end.
+
+  Definition encode_word_Impl (w : word sz) (ce : CacheEncode) : B * CacheEncode := (encode_word' sz w, addE ce sz).
+
+  Definition encode_word_Spec (w : word sz) (ce : CacheEncode) : Comp (B * CacheEncode) :=
+    ret (encode_word' sz w, addE ce sz).
+
+  Fixpoint decode_word' (s : nat) (b : B) : option (word s * B) :=
+    match s with
+    | O => Some (WO, b)
+    | S s' =>
+      `(c, b') <- transform_pop_opt b;
+      `(w, bx) <- decode_word' s' b';
+       Some (WS c w, bx)
+    end.
+
+  Definition decode_word (b : B) (cd : CacheDecode) : option (word sz * B * CacheDecode) :=
+    Ifopt decode_word' sz b as decoded Then Some (decoded, addD cd sz) Else None.
+
+  Theorem Word_decode_correct
+          {P : CacheDecode -> Prop}
+          (P_OK : cache_inv_Property P (fun P => forall b cd, P cd -> P (addD cd b)))
+    :
+      encode_decode_correct_f cache transformer (fun _ => True)
+                              (fun _ _ => True)
+                              encode_word_Spec decode_word P.
+  Proof.
+    unfold encode_decode_correct_f, encode_word_Spec, decode_word; split.
+    - intros env env' xenv w w' ext Eeq _ _ Penc.
+      computes_to_inv; injections.
+      generalize dependent sz.
+      induction w; simpl in *.
+      { eexists; split; eauto; try rewrite !transform_id_left;
+        eauto using add_correct. }
+      { rewrite transform_push_step_opt.
+        rewrite transform_push_pop_opt.
+        destruct_ex; intuition.
+        destruct (decode_word' n (transform (encode_word' n w) ext)) as [ [? ?] | ] eqn: ?; simpl in *; try discriminate.
+        injections; eexists; split; eauto using add_correct.
+        rewrite Heqo; simpl; f_equal.
+      }
+    - intros.
+      destruct (decode_word' sz bin)
+        as [ [? ?] | ] eqn: ?; simpl in *; try discriminate.
+      injections.
+      generalize dependent bin.
+      induction data; simpl in *.
+      { intros; computes_to_inv; intros; injection Heqo; clear Heqo;
+        intros; subst.
+        repeat eexists; eauto; try rewrite !transform_id_left;
+        eauto using add_correct.
+      }
+      { intros; intuition.
+        destruct (transform_pop_opt bin) as [ [? ?] | ] eqn: ? ;
+          simpl in *; try discriminate.
+        destruct (decode_word' n b1) as [ [? ? ] | ] eqn: ? ;
+          simpl in *; try discriminate.
+        injection Heqo; intros; subst.
+        apply Eqdep_dec.inj_pair2_eq_dec in H2; subst.
+        eapply IHdata in Heqo1.
+        intuition; destruct_ex; intuition; subst.
+        computes_to_inv; injections.
+        eexists; eexists; repeat split.
+        setoid_rewrite transform_push_step_opt.
+        eapply transform_pop_opt_inj; eauto.
+        rewrite transform_push_pop_opt; reflexivity.
+        apply add_correct; eauto.
+        eapply Peano_dec.eq_nat_dec.
+      }
+  Qed.
+
+  Lemma decode_word'_le
+    : forall (a : word sz) (b' b1 : B),
+      decode_word' _ b1  = Some (a, b') -> le_B b' b1.
+  Proof.
+    induction a; simpl.
+    - intros; injections; unfold le_B; omega.
+    - intros; simpl.
+      destruct (transform_pop_opt b1) as [ [? ?] | ] eqn: ? ;
+        subst; simpl in *; try discriminate.
+      destruct (decode_word' n b2) as [ [? ?] | ] eqn: ? ;
+        subst; simpl in *; try discriminate.
+      injection H; intros; subst; unfold le_B in *.
+      pose proof (IHa b' b2).
+      rewrite Heqo0 in H0; simpl in *.
+      apply Eqdep_dec.inj_pair2_eq_dec in H1; subst.
+      pose proof (H0 (eq_refl _)).
+      eapply measure_pop_Some in Heqo; subst.
+      omega.
+      eapply Peano_dec.eq_nat_dec.
+  Qed.
+
+  Lemma decode_word_le
+    : forall (cd : CacheDecode) (a : word sz)
+             (b' b1 : B) (cd' : CacheDecode),
+      decode_word b1 cd = Some (a, b', cd') -> le_B b' b1.
+  Proof.
+    unfold decode_word.
+    intros; destruct (decode_word' sz b1) as [ [? ?] | ] eqn: ? ;
+      subst; simpl in *; try discriminate.
+    injections.
+    eapply decode_word'_le; eauto.
+  Qed.
+
+  Lemma decode_word'_lt
+    : forall (a : word (S sz)) (b' b1 : B),
+      decode_word' _ b1 = Some (a, b') -> lt_B b' b1.
+  Proof.
+    simpl; intros; injections; unfold lt_B.
+    destruct (transform_pop_opt b1) as [ [? ?] | ] eqn: ? ;
+      subst; simpl in *; try discriminate.
+    apply measure_pop_Some in Heqo; subst.
+    destruct (decode_word' sz b0) as [ [? ?] | ] eqn: ? ;
+        subst; simpl in *; try discriminate.
+    eapply decode_word'_le in Heqo0; injections.
+    rewrite Heqo.
+    unfold le_B in *.
+    pose proof (T_measure_gt_0 b).
+    omega.
+  Qed.
+
+  Lemma decode_word_lt
+    : forall (cd : CacheDecode) (a : word (S sz))
+             (b' b1 : B) (cd' : CacheDecode),
+      Ifopt decode_word' _ b' as decoded Then Some (decoded, addD cd (S sz)) Else None = Some (a, b1, cd') -> lt_B b1 b'.
+  Proof.
+    intros; destruct (decode_word' (S sz) b') as [ [? ?] | ] eqn: ? ;
+    try eapply decode_word'_lt in Heqo;
+      simpl in *; try (subst; discriminate).
+    injections.
+    unfold lt_B in *.
+    omega.
+  Qed.
+
+  Definition encode_unused_word_Spec' (sz : nat)
+             (_ : unit) (ctx : CacheEncode) :=
+    (w <- { w : word sz | True};
+       ret (encode_word' sz w, addE ctx sz))%comp.
+
+  Definition encode_unused_word_Spec
+             (sz : nat)
+             (ctx : CacheEncode) :=
+    encode_unused_word_Spec' sz tt ctx.
+
+  Fixpoint transformer_get_word {B}
+           {transformer : Transformer B}
+           {transformer_opt : TransformerUnitOpt transformer bool}
+           (sz : nat)
+           (b : B)
+    : option (word sz) :=
+    match sz with
+    | 0 => Some WO
+    | S sz' =>
+      match transform_pop_opt b with
+      | Some (v, b') =>
+        match transformer_get_word sz' b' with
+        | Some w => Some (WS v w)
+        | _ => None
+        end
+      | _ => None
+      end
+    end.
+
+  Fixpoint transformer_pop_word
+         (sz : nat)
+         (b : B)
+  : option (word sz * B) :=
+  match sz with
+  | 0 => Some (WO, b)
+  | S sz' =>
+    match transform_pop_opt b with
+    | Some (v, b') =>
+      match transformer_pop_word sz' b' with
+      | Some (w', b'') => Some (WS v w', b'')
+      | _ => None
+      end
+    | _ => None
+    end
+  end.
+
+  Lemma transformer_pop_word_eq_decode_word' : 
+    forall (sz : nat)
+           (b : B),
+      transformer_pop_word sz b = decode_word' sz b.
+  Proof.
+    induction sz0; simpl; eauto.
+  Qed.  
+
+  Lemma transformer_pop_encode_word'
+        (sz' : nat)
+    : forall (w : word sz') (ext : B),
+      transformer_pop_word sz' (transform (encode_word' _ w) ext) = Some (w, ext).
+  Proof.
+    induction sz'; simpl; intros.
+    - rewrite (shatter_word w); eauto.
+      unfold encode_word'; rewrite transform_id_left; reflexivity.
+    - rewrite (shatter_word w); simpl.
+      rewrite transform_push_step_opt, transform_push_pop_opt.
+      rewrite IHsz'; eauto.
+  Qed.
+
+  Definition decode_unused_word' (s : nat) (b : B) : option (unit * B) :=
+    Ifopt transformer_pop_word s b as b' Then Some (tt, snd b') Else None.
+
+  Definition decode_unused_word (sz' : nat)
+             (b : B) (cd : CacheDecode) : option (unit * B * CacheDecode) :=
+    Ifopt decode_unused_word' sz' b as decoded Then Some (decoded, addD cd sz') Else None.
+
+  Theorem unused_word_decode_correct sz'
+          {P : CacheDecode -> Prop}
+          (P_OK : cache_inv_Property P (fun P => forall b cd, P cd -> P (addD cd b)))
+    :
+      encode_decode_correct_f cache transformer (fun _ => True)
+                              (fun _ _ => True)
+                              (encode_unused_word_Spec' sz') (decode_unused_word sz') P.
+  Proof.
+    unfold encode_decode_correct_f, encode_unused_word_Spec', decode_unused_word; split.
+    - intros env env' xenv w w' ext Eeq _ _ Penc.
+      computes_to_inv; injections.
+      unfold decode_unused_word'.
+      rewrite transformer_pop_encode_word'; simpl.
+      destruct w.
+      eexists; split; eauto using add_correct.
+    - intros.
+      destruct (decode_unused_word' sz' bin)
+        as [ [? ?] | ] eqn: ?; simpl in *; try discriminate.
+      injections.
+      destruct data.
+      generalize dependent bin.
+      induction sz'; simpl in *.
+      { intros; computes_to_inv; intros; injection Heqo; clear Heqo;
+        intros; subst.
+        repeat eexists; eauto; try rewrite !transform_id_left;
+        eauto using add_correct.
+        instantiate (1 := WO); simpl.
+        rewrite !transform_id_left; eauto.
+      }
+      { intros; intuition.
+        unfold decode_unused_word' in Heqo.
+        simpl in Heqo.
+        destruct (transform_pop_opt bin) as [ [? ?] | ] eqn: ? ;
+          simpl in *; try discriminate.
+        destruct (transformer_pop_word sz' b0) as [ [? ?] | ] eqn: ? ;
+          simpl in *; try discriminate.
+        injection Heqo; intros; subst.
+        destruct (IHsz' b0).
+        unfold decode_unused_word'; rewrite Heqo1; simpl; eauto.
+        intuition; destruct_ex; intuition; subst.
+        computes_to_inv; injections.
+        eexists; eexists; repeat split.
+        repeat computes_to_econstructor; eauto.
+        instantiate (1 := WS b v); simpl.
+        setoid_rewrite transform_push_step_opt.
+        eapply transform_pop_opt_inj; eauto.
+        rewrite transform_push_pop_opt; reflexivity.
+        apply add_correct; eauto.
+      }
+  Qed.
+
+End Word.
+
